WIP: Add more graph lemmas

graph.v
@@ -1,4 +1,4 @@
-From iris.algebra Require Import base.
+From iris.algebra Require Import base cmra gmap.
 From iris.prelude Require Import gmap mapset.
 
 (* Definition of a doubly branching graphs and tree. *)
@@ -31,21 +31,19 @@ Section Graphs.
 
   (* For some reason, perhaps a bug, type class inference can't find
 gmap_lookup instance when defining an inductive! *)
-  Local Notation glu := (@lookup _ _ Graph (@gmap_lookup _ _ _ _)).
 
   Inductive Path g (P : bool → bool) (x : T) : T → Type :=
-  | Path_O : ∀ m l r, glu x g = Some (m, (l, r)) → P m → Path g P x x
+  | Path_O : ∀ m l r, g !! x = Some (m, (l, r)) → P m → Path g P x x
   | Path_Sl : ∀ y z m r,
-      Path g P x y → bool_decide (glu y g = Some (m, (Some z, r)))
+      Path g P x y → bool_decide (g !! y = Some (m, (Some z, r)))
       → P m → Path g P x z
   | Path_Sr : ∀ y z m l,
-      Path g P x y → bool_decide (glu y g = Some (m, (l, Some z)))
+      Path g P x y → bool_decide (g !! y = Some (m, (l, Some z)))
       → P m → Path g P x z.
 
-
   (* The fragment of g satisfying P is a connected graph and x is in there. *)
-  Definition connected (g : Graph) P (x : T) :=
-    ∀ y, y ∈ dom (gset _) g → Path g P x y.
+  Definition connected (g : Graph) (P : bool → bool) (x : T) :=
+    ∀ y m x1 x2, g !! y = Some (m, (x1, x2)) → P m → Path g P x y.
 
   (* The fragment of g satisfying P is a tree with root x. *)
   Record tree (g : Graph) P (x : T) :=
@@ -74,5 +72,175 @@ immediately reachable from nodes in X. *)
                           ) (map_to_list g))
                    then Some (x.1, ()) else None
             ) (map_to_list g))).
+
+  Record maximal_marked_tree g x :=
+    {
+      mmtr_tree : tree g (λ m, m) x;
+      mmtr_maximal : front g (marked g) ⊆ (marked g)
+    }.
+
+  Definition combine_node_data
+             (x y : option (bool * (option T * option T))) :
+    option (bool * (option T * option T))
+    :=
+      match x, y with
+      | Some (false, (xl, xr)), Some (false, (yl, yr)) =>
+                         if bool_decide (xl = yl ∧ xr = yr) then
+                           Some (false, (xl, xr))
+                         else
+                           None
+      | Some (true, (xl, xr)), Some (false, (yl, yr)) => Some (true, (xl, xr))
+      | Some (false, (xl, xr)), Some (true, (yl, yr)) => Some (true, (yl, yr))
+      | _, _ => None
+      end.
+
+  Instance combine_node_data_DiagNone : DiagNone combine_node_data := eq_refl.
+
+  Definition combine_graphs g1 g2 : option Graph :=
+    if mapset_disjoint_dec (marked g1) (marked g2) then
+      Some (merge combine_node_data g1 g2)
+    else
+      None.
+
+  Lemma combine_graphs_comm g1 g2 : combine_graphs g1 g2 = combine_graphs g2 g1.
+  Proof.
+    unfold combine_graphs; repeat destruct mapset_disjoint_dec;
+      trivial;
+      try match goal with
+            H : ¬ _ ⊥ _ |- _ => contradict H; apply disjoint_sym; trivial
+          end.
+    f_equal.
+    apply merge_comm.
+    - typeclasses eauto.
+    - intros x.
+      destruct (@lookup _ _ (gmap _ _) _ x g1) as [[[] [x1l x1r]]|];
+        destruct (@lookup _ _ (gmap _ _) _ x g2) as [[[] [x2l x2r]]|]; cbn;
+          trivial.
+      repeat unfold bool_decide; repeat destruct option_eq_dec; cbn in *;
+        repeat match goal with
+                 H : ?A = _ |- _ => subst A
+               end; trivial; try tauto.
+  Qed.
+
+  Lemma combine_graphs_dom_stable g1 g2 g3 :
+    dom (gset _) g1 = dom (gset _) g2 →
+    (∀ x l1 l2 r1 r2,
+        @lookup _ _ (gmap _ _) _ x g1 = Some (false, (l1, r1)) →
+        @lookup _ _ (gmap _ _) _ x g2 = Some (false, (l2, r2)) →
+        l1 = l2 ∧ r1 = r2
+    ) → combine_graphs g1 g2 = Some g3 → dom (gset _) g3 = dom (gset _) g1.
+  Proof.
+    intros H1 H2 H3.
+    (apply mapset_eq => x);
+      set (H1' := proj1 (mapset_eq _ _) H1 x); clearbody H1';
+        destruct H1' as [H11 H12].
+    specialize (H2 x).
+    unfold combine_graphs in H3; destruct mapset_disjoint_dec as [d|nd];
+      inversion H3; subst; clear H3.
+    set (d' := proj1 (elem_of_disjoint _ _) d x); clearbody d'; clear d.
+    revert H11 H12 d';
+      rewrite /dom /gset_dom /mapset_dom ?elem_of_mapset_dom_with => H11 H12 d'.
+    rewrite lookup_merge. split; intros [y [Hy _]].
+    - destruct (@lookup _ _ (gmap _ _) _ x g1) as [[[] [x1l x1r]]|];
+        destruct (@lookup _ _ (gmap _ _) _ x g2) as [[[] [x2l x2r]]|]; cbn in *;
+          trivial; try inversion Hy; eauto.
+    - destruct (@lookup _ _ (gmap _ _) _ x g1) as [[[] [x1l x1r]]|];
+        destruct (@lookup _ _ (gmap _ _) _ x g2) as [[[] [x2l x2r]]|]; cbn in *;
+      try (inversion Hy; fail); eauto.
+      + exfalso; apply d'; eauto.
+      + unfold bool_decide; repeat destruct option_eq_dec; subst; cbn; eauto;
+        edestruct H2 as [H21 H22]; eauto; try tauto.
+  Qed.
+
+  Lemma combine_graphs_marked_eq_union g1 g2 g3 :
+    dom (gset _) g1 = dom (gset _) g2 →
+    (∀ x l1 l2 r1 r2,
+        @lookup _ _ (gmap _ _) _ x g1 = Some (false, (l1, r1)) →
+        @lookup _ _ (gmap _ _) _ x g2 = Some (false, (l2, r2)) →
+        l1 = l2 ∧ r1 = r2
+    ) → combine_graphs g1 g2 = Some g3 → marked g3 = (marked g1) ∪ (marked g2).
+  Proof.
+    intros H1 H2 H3.
+    apply mapset_eq => x; split => Hx.
+    - unfold combine_graphs in H3; destruct mapset_disjoint_dec as [d|nd];
+      inversion H3; subst; clear H3.
+      apply elem_of_mapset_dom_with in Hx. destruct Hx as [y [Hy1 Hy2]].
+      rewrite lookup_merge in Hy1.
+      apply elem_of_union.
+      unfold marked; rewrite ?elem_of_mapset_dom_with.
+      destruct (@lookup _ _ (gmap _ _) _ x g1) as [[[] [x1l x1r]]|];
+        destruct (@lookup _ _ (gmap _ _) _ x g2) as [[[] [x2l x2r]]|];
+        (try (inversion Hy1; fail)); cbn in Hy1; cbn; eauto.
+      unfold bool_decide in Hy1; repeat destruct option_eq_dec;
+        subst; cbn in *; try discriminate; eauto.
+    - set (H4 := combine_graphs_dom_stable _ _ _ H1 H2 H3);
+        clearbody H4.
+      unfold combine_graphs in H3; destruct mapset_disjoint_dec as [d|nd];
+        inversion H3; subst; clear H3.
+      apply elem_of_union in Hx.
+      revert Hx; rewrite ?elem_of_mapset_dom_with => Hx.
+      set (H5 := proj1 (mapset_eq _ _) H4 x). destruct H5 as [H51 H52].
+      revert H51 H52. rewrite ?elem_of_dom. unfold is_Some.
+      set (H6 := proj1 (mapset_eq _ _) (eq_trans H4 H1) x).
+      destruct H6 as [H61 H62]. revert H61 H62. rewrite ?elem_of_dom.
+      unfold is_Some.
+      set (d' := proj1 (elem_of_disjoint _ _) d). specialize (d' x).
+      revert d'; rewrite ?elem_of_mapset_dom_with.
+      clear H1 H4 d. specialize (H2 x).
+      rewrite ?lookup_merge. intros d H61 H62 H41 H42.
+      destruct (@lookup _ _ (gmap _ _) _ x g1) as [[[] [x1l x1r]]|];
+        destruct (@lookup _ _ (gmap _ _) _ x g2) as [[[] [x2l x2r]]|]; cbn in *;
+          eauto;
+          try match goal with
+            H : _ → _ |- _ =>
+            match type of H with
+              ?A → ?B => cut (B → False);
+                          [let H := fresh in intros H; exfalso; apply H; eauto|
+                           clear; let H := fresh in intros H; firstorder]; fail
+            end
+          end.
+      + exfalso. destruct Hx as [[y [Hy1 Hy2]]|[y [Hy1 Hy2]]]; inversion Hy1;
+                   subst; cbn in *; trivial.
+      + destruct Hx as [[y [Hy1 Hy2]]|[y [Hy1 Hy2]]]; discriminate.
+  Qed.
+
+  Lemma combine_graphs_marked_subseteq_union g1 g2 g3 :
+    combine_graphs g1 g2 = Some g3 → marked g3 ⊆ (marked g1) ∪ (marked g2).
+  Proof.
+    intros H1.
+    apply elem_of_subseteq => x Hx.
+    unfold combine_graphs in H1; destruct mapset_disjoint_dec as [d|nd];
+      inversion H1; subst; clear H1.
+    apply elem_of_mapset_dom_with in Hx. destruct Hx as [y [Hy1 Hy2]].
+    rewrite lookup_merge in Hy1.
+    apply elem_of_union.
+    unfold marked; rewrite ?elem_of_mapset_dom_with.
+    destruct (@lookup _ _ (gmap _ _) _ x g1) as [[[] [x1l x1r]]|];
+      destruct (@lookup _ _ (gmap _ _) _ x g2) as [[[] [x2l x2r]]|];
+      (try (inversion Hy1; fail)); cbn in Hy1; cbn; eauto.
+    unfold bool_decide in Hy1; repeat destruct option_eq_dec;
+      subst; cbn in *; try discriminate; eauto.
+  Qed.
+
+  Lemma combine_maximal_marked_trees_both g1 g2 x x1 x2
+        (Hg1x : (g1 !! x = Some (false, (Some x1, Some x2))))
+        (Hg2x : (g2 !! x = Some (false, (Some x1, Some x2))))
+        (t1 : maximal_marked_tree g1 x1)
+        (t2 : maximal_marked_tree g1 x2)
+        g3
+        (Hc : combine_graphs g1 g2 = Some g3)
+    : maximal_marked_tree (<[x := (true, (Some x1, Some x2))]> g3) x.
+  Proof.
+    repeat constructor.
+    - intros w b ? ? H1 H2.
+      rewrite insert_union_singleton_l in H1. 
+      set (Hu := combine_graphs_marked_subseteq_union _ _ _ Hc); clearbody Hu.
+      unfold combine_graphs in Hc; destruct mapset_disjoint_dec as [d|nd];
+        inversion Hc; subst; clear Hc.
+      admit.
+    - intros w H1 p p'.
+      admit.
+    - admit.
+  Admitted.
 
 End Graphs.
